Add external value types
This makes things slightly messy, but it does seem to work.

We have one serious annoyance, which is that in order to generically
prove that the zero value has the right type, I had to make the zero
value for external values type-check. This breaks the abstraction we
wanted; really, in the model we shouldn't support taking the zero value
of an external type (which is annoying to change now, but it should
work).

src/go_lang/ffi/disk.v
@@ -31,18 +31,38 @@ Proof.
                    end) _); by intros [].
 Qed.
 
-Definition disk_op : ext_op.
+Inductive Disk_val := .
+Instance eq_Disk_val : EqDecision Disk_val.
 Proof.
-  refine (mkExtOp DiskOp _ _).
+  intros [].
 Defined.
 
+Instance eq_Disk_fin : Countable Disk_val.
+Proof.
+  refine {| encode := fun (x: Disk_val) => match x with end;
+            decode := fun x => None; |}.
+  intros [].
+Qed.
+
+Definition disk_op : ext_op.
+Proof.
+  refine (mkExtOp DiskOp _ _ Disk_val _ _).
+Defined.
+
+Instance disk_val_ty: val_types :=
+  {| ext_tys := Empty_set; |}.
+
 Definition disk_ty: ext_types disk_op :=
-  {| get_ext_tys (op: @external disk_op) :=
+  {| val_tys := disk_val_ty;
+     val_ty_def x := match x with end;
+     get_ext_tys (op: @external disk_op) :=
        match op with
     | ReadOp => (uint64T, arrayT byteT)
     | WriteOp => (prodT uint64T (arrayT byteT), unitT)
     | SizeOp => (unitT, uint64T)
        end; |}.
+
+Local Canonical Structure disk_ty.
 
 Definition block_bytes: nat := N.to_nat 4096.
 Definition BlockSize {ext: ext_op}: val := #4096.
