src/go_lang/basic_triples.v
@@ -19,6 +19,7 @@ Set Printing Projections.
 
 Section heap.
 Context `{ffi_sem: ext_semantics} `{!ffi_interp ffi} `{!heapG Σ}.
+Context {ext_ty: ext_types ext}.
 Implicit Types P Q : iProp Σ.
 Implicit Types Φ : val → iProp Σ.
 Implicit Types Δ : envs (uPredI (iResUR Σ)).
