src/go_lang/lang.v
@@ -68,6 +68,10 @@ Class ext_op :=
       external: Set;
       external_eq_dec :> EqDecision external;
       external_countable :> Countable external;
+
+      ext_val: Type;
+      ext_val_eq_dec :> EqDecision ext_val;
+      ext_val_countable :> Countable ext_val;
     }.
 
 Class ffi_model :=
@@ -78,8 +82,8 @@ Class ffi_model :=
 
 Section external.
 
-(* these are just codes for external operations (which all take a single val as
-   an argument and evaluate to a value) *)
+(* these are codes for external operations (which all take a single val as an
+   argument and evaluate to a value) and data for external values *)
 Context {ext : ext_op}.
 
 (** We have a notion of "poison" as a variant of unit that may not be compared
@@ -152,6 +156,7 @@ with val :=
   | PairV (v1 v2 : val)
   | InjLV (v : val)
   | InjRV (v : val)
+  | ExtV (x : ext_val)
 .
 
 Bind Scope expr_scope with expr.
@@ -285,7 +290,7 @@ Definition val_is_unboxed (v : val) : Prop :=
 Global Instance lit_is_unboxed_dec l : Decision (lit_is_unboxed l).
 Proof. destruct l; simpl; exact (decide _). Defined.
 Global Instance val_is_unboxed_dec v : Decision (val_is_unboxed v).
-Proof. destruct v as [ | | | [] | [] ]; simpl; exact (decide _). Defined.
+Proof. destruct v as [ | | | [] | [] | ]; simpl; exact (decide _). Defined.
 
 (** We just compare the word-sized representation of two values, without looking
 into boxed data.  This works out fine if at least one of the to-be-compared
@@ -385,6 +390,7 @@ Proof using ext.
         cast_if_and (decide (e1 = e1')) (decide (e2 = e2'))
       | InjLV e, InjLV e' => cast_if (decide (e = e'))
       | InjRV e, InjRV e' => cast_if (decide (e = e'))
+      | ExtV x, ExtV x' => cast_if (decide (x = x'))
       | _, _ => right _
       end
         for go); try (clear go gov; abstract intuition congruence).
@@ -402,6 +408,7 @@ Proof using ext.
        cast_if_and (decide (e1 = e1')) (decide (e2 = e2'))
      | InjLV e, InjLV e' => cast_if (decide (e = e'))
      | InjRV e, InjRV e' => cast_if (decide (e = e'))
+     | ExtV x, ExtV x' => cast_if (decide (x = x'))
      | _, _ => right _
      end); try abstract intuition congruence.
 Defined.
@@ -521,6 +528,7 @@ Inductive basic_type :=
   | bin_opVal (op:bin_op)
   | primOpVal (op:prim_op')
   | externOp (op:external)
+  | extVal (x:ext_val)
 .
 
 Instance basic_type_eq_dec : EqDecision basic_type.
@@ -535,7 +543,8 @@ Proof.
                               | un_opVal op => inr (inr (inr (inr (inl op))))
                               | bin_opVal op => inr (inr (inr (inr (inr (inl op)))))
                               | primOpVal op => inr (inr (inr (inr (inr (inr (inl op))))))
-                              | externOp op => inr (inr (inr (inr (inr (inr (inr op))))))
+                              | externOp op => inr (inr (inr (inr (inr (inr (inr (inl op)))))))
+                              | extVal x => inr (inr (inr (inr (inr (inr (inr (inr x)))))))
                               end)
                          (λ x, match x with
                               | inl s => stringVal s
@@ -545,7 +554,8 @@ Proof.
                               | inr (inr (inr (inr (inl op)))) => un_opVal op
                               | inr (inr (inr (inr (inr (inl op))))) => bin_opVal op
                               | inr (inr (inr (inr (inr (inr (inl op)))))) => primOpVal op
-                              | inr (inr (inr (inr (inr (inr (inr op)))))) => externOp op
+                              | inr (inr (inr (inr (inr (inr (inr (inl op))))))) => externOp op
+                              | inr (inr (inr (inr (inr (inr (inr (inr x))))))) => extVal x
                                end) _); by intros [].
 Qed.
 
@@ -601,6 +611,7 @@ Proof using ext.
      | PairV v1 v2 => GenNode 1 [gov v1; gov v2]
      | InjLV v => GenNode 2 [gov v]
      | InjRV v => GenNode 3 [gov v]
+     | ExtV x => GenNode 4 [GenLeaf $ extVal x]
      end
    for go).
  set (dec :=
@@ -637,6 +648,7 @@ Proof using ext.
      | GenNode 1 [v1; v2] => PairV (gov v1) (gov v2)
      | GenNode 2 [v] => InjLV (gov v)
      | GenNode 3 [v] => InjRV (gov v)
+     | GenNode 4 [GenLeaf (extVal x)] => ExtV x
      | _ => LitV LitUnit (* dummy *)
      end
    for go).
